#

A=x^2+4y^2,B=2x^2-y^2\
x=?

1. A+x=B
2. 2x-3A=2B+x

1) A+x=B\
= (2x^2-y^2)-(x^2+4y^2)\
= (2+1)x^2-(4-3)y^2\
= x^2-3y^2

2) 2x-3A=2B+x\
2x-x=3A+2B\
x=3A+2B\
x=3(x^2+4y^2)+2(2x^2-y^2)\
x=3x^2+12y^2+4x^2-2y^2\
x=(3+4)x^2+(12-2)y^2\
x=7x^3+10y^2

## 다항식의 곱셈

$(x+2y)(2x+3y)$\
= $x(2x+3y)+2y(2x+3y)$\
= $2x^2+3xy+4xy+6y^2$\
= $2x^2+7xy+6y^2$

$(x-3)(x+2)(x+3)$

1. $(x-3)(x+3)$
2. $(x+2)$

1) = $x(x+3)-3(x+3)$\
= $x^2+3x-3x-9$

2) $(x^2-9)*(x+2)$\
$x^2(x+2)+-9(x+2)$\
$x^3+2x^2-9x-18$

## bruh so many math

- $(a-b)^2=a^2-2ab+b^2$
- $(a+b)^2=a^2+2ab+b^2$
- $(a+b+c)^2=a^2+b^2+c^2+2ab+2bc+2ca$
- $(a+b)^3=a^3+3a^2b+3ab^2+b^3$
- $(a-b)^3=a^3+3a^2b+3ab^2-b^3$
- $(a+b)(a^2-ab+b^2)=a^3-b^3$
- $(x+a)(x+b)=x^2+(a+b)x+ab$
- $(ax+b)(cx+d)=acx^2+(ad+bc)x+bd$
